Coinduction for isim

src/Weakest.v
@@ -1,6 +1,7 @@
 From sflib Require Import sflib.
 From Paco Require Import paco.
 From Fairness Require Import PCM ITreeLib IProp IPM ModSim ModSimNat.
+Require Import Program.
 
 Set Implicit Arguments.
 
@@ -43,7 +44,7 @@ Section SIM.
   Variable tid: thread_id.
   Variable I: shared_rel.
 
-  Let rel := (forall R_src R_tgt (Q: R_src -> R_tgt -> shared_rel), itree srcE R_src -> itree tgtE R_tgt -> shared_rel).
+  Let rel := (forall R_src R_tgt (Q: R_src -> R_tgt -> shared_rel), bool -> bool -> itree srcE R_src -> itree tgtE R_tgt -> shared_rel).
 
   Let coind :=  (bool * bool * rel * rel)%type.
 
@@ -70,21 +71,42 @@ Section SIM.
     (fun R_src R_tgt RR ps pt r_ctx itr_src itr_tgt '(ths, im_src, im_tgt, st_src, st_tgt) => exists r_own,
          (<<WF: URA.wf (r_own ⋅ r_ctx)>>) /\
            (<<SAT: @r _ _ (fun r_src r_tgt ths im_src im_tgt st_src st_tgt =>
-                             @iProp_intro _ (fun r_own => forall (r_ctx: Σ) (WF: URA.wf (r_own ⋅ r_ctx)),                                                                                     RR r_src r_tgt r_ctx (ths, im_src, im_tgt, st_src, st_tgt)) _) itr_src itr_tgt ths im_src im_tgt st_src st_tgt r_own>>)).
+                             @iProp_intro _ (fun r_own => forall (r_ctx: Σ) (WF: URA.wf (r_own ⋅ r_ctx)),                                                                                     RR r_src r_tgt r_ctx (ths, im_src, im_tgt, st_src, st_tgt)) _) ps pt itr_src itr_tgt ths im_src im_tgt st_src st_tgt r_own>>)).
   Next Obligation.
   Proof.
     i. ss. i. eapply H.
     eapply URA.wf_extends; eauto. eapply URA.extends_add; eauto.
   Qed.
 
-  Program Definition isim: coind -> rel :=
+  Variant unlift2 (r: rel):
+    forall R_src R_tgt (RR: R_src -> R_tgt -> Σ ->
+                            (TIdSet.t *
+                               (@imap ident_src wf_src) *
+                               (@imap (sum_tid ident_tgt) nat_wf) *
+                               state_src *
+                               state_tgt) -> Prop),
+      bool -> bool -> Σ -> itree srcE R_src -> itree tgtE R_tgt ->
+      (TIdSet.t *
+         (@imap ident_src wf_src) *
+         (@imap (sum_tid ident_tgt) nat_wf) *
+         state_src *
+         state_tgt) -> Prop :=
+    | unlift2_intro
+        R_src R_tgt Q ps pt itr_src itr_tgt ths im_src im_tgt st_src st_tgt r_ctx r_own
+        (REL: r R_src R_tgt Q ps pt itr_src itr_tgt ths im_src im_tgt st_src st_tgt r_own)
+        (WF: URA.wf (r_own ⋅ r_ctx))
+      :
+      unlift2 r (liftRR Q) ps pt r_ctx itr_src itr_tgt (ths, im_src, im_tgt, st_src, st_tgt)
+  .
+
+  Program Definition isim: rel -> rel -> rel :=
     fun
-      '(ps, pt, r, g)
-      R_src R_tgt Q itr_src itr_tgt ths im_src im_tgt st_src st_tgt =>
+      r g
+      R_src R_tgt Q ps pt itr_src itr_tgt ths im_src im_tgt st_src st_tgt =>
       iProp_intro
         (fun r_own =>
            forall r_ctx (WF: URA.wf (r_own ⋅ r_ctx)),
-             gpaco9 gf (cpn9 gf) (@unlift r) (@unlift g) _ _ (liftRR Q) ps pt r_ctx itr_src itr_tgt (ths, im_src, im_tgt, st_src, st_tgt)) _.
+             gpaco9 gf (cpn9 gf) (@unlift2 r) (@unlift2 g) _ _ (liftRR Q) ps pt r_ctx itr_src itr_tgt (ths, im_src, im_tgt, st_src, st_tgt)) _.
   Next Obligation.
   Proof.
     ii. ss. eapply H.
@@ -103,8 +125,8 @@ Section SIM.
         itr_src itr_tgt ths im_src im_tgt st_src st_tgt
     :
     bi_entails
-      (isim (ps, pt, r, g) Q0 itr_src itr_tgt ths im_src im_tgt st_src st_tgt)
-      (isim (ps, pt, r, g) Q1 itr_src itr_tgt ths im_src im_tgt st_src st_tgt)
+      (isim r g Q0 ps pt itr_src itr_tgt ths im_src im_tgt st_src st_tgt)
+      (isim r g Q1 ps pt itr_src itr_tgt ths im_src im_tgt st_src st_tgt)
   .
   Proof.
     rr. autorewrite with iprop. i.
@@ -125,8 +147,8 @@ Section SIM.
         itr_src itr_tgt ths im_src im_tgt st_src st_tgt
     :
     bi_entails
-      (#=> (isim (ps, pt, r, g) Q itr_src itr_tgt ths im_src im_tgt st_src st_tgt))
-      (isim (ps, pt, r, g) Q itr_src itr_tgt ths im_src im_tgt st_src st_tgt)
+      (#=> (isim r g Q ps pt itr_src itr_tgt ths im_src im_tgt st_src st_tgt))
+      (isim r g Q ps pt itr_src itr_tgt ths im_src im_tgt st_src st_tgt)
   .
   Proof.
     rr. autorewrite with iprop. i.
@@ -141,8 +163,8 @@ Section SIM.
         (PT: pt0 = true -> pt1 = true)
     :
     bi_entails
-      (isim (ps0, pt0, r, g) Q itr_src itr_tgt ths im_src im_tgt st_src st_tgt)
-      (isim (ps1, pt1, r, g) Q itr_src itr_tgt ths im_src im_tgt st_src st_tgt)
+      (isim r g Q ps0 pt0 itr_src itr_tgt ths im_src im_tgt st_src st_tgt)
+      (isim r g Q ps1 pt1 itr_src itr_tgt ths im_src im_tgt st_src st_tgt)
   .
   Proof.
     rr. autorewrite with iprop. i.
@@ -156,8 +178,8 @@ Section SIM.
     :
     bi_entails
       ((∀ r_src r_tgt ths im_src im_tgt st_src st_tgt,
-           ((Q0 r_src r_tgt ths im_src im_tgt st_src st_tgt) -∗ (Q1 r_src r_tgt ths im_src im_tgt st_src st_tgt))) ** (isim (ps, pt, r, g) Q0 itr_src itr_tgt ths im_src im_tgt st_src st_tgt))
-      (isim (ps, pt, r, g) Q1 itr_src itr_tgt ths im_src im_tgt st_src st_tgt)
+           ((Q0 r_src r_tgt ths im_src im_tgt st_src st_tgt) -∗ (Q1 r_src r_tgt ths im_src im_tgt st_src st_tgt))) ** (isim r g Q0 ps pt itr_src itr_tgt ths im_src im_tgt st_src st_tgt))
+      (isim r g Q1 ps pt itr_src itr_tgt ths im_src im_tgt st_src st_tgt)
   .
   Proof.
     rr. autorewrite with iprop. i.
@@ -192,9 +214,9 @@ Section SIM.
         ths im_src im_tgt st_src st_tgt
     :
     bi_entails
-      (isim (ps, pt, r, g) (fun s_src s_tgt ths im_src im_tgt st_src st_tgt =>
-                   isim (false, false, r, g) Q (ktr_src s_src) (ktr_tgt s_tgt) ths im_src im_tgt st_src st_tgt) itr_src itr_tgt ths im_src im_tgt st_src st_tgt)
-      (isim (ps, pt, r, g) Q (itr_src >>= ktr_src) (itr_tgt >>= ktr_tgt) ths im_src im_tgt st_src st_tgt)
+      (isim r g (fun s_src s_tgt ths im_src im_tgt st_src st_tgt =>
+                   isim r g Q false false (ktr_src s_src) (ktr_tgt s_tgt) ths im_src im_tgt st_src st_tgt) ps pt itr_src itr_tgt ths im_src im_tgt st_src st_tgt)
+      (isim r g Q ps pt (itr_src >>= ktr_src) (itr_tgt >>= ktr_tgt) ths im_src im_tgt st_src st_tgt)
   .
   Proof.
     rr. autorewrite with iprop. i.
@@ -215,8 +237,8 @@ Section SIM.
         itr_src itr_tgt ths im_src im_tgt st_src st_tgt
     :
     bi_entails
-      (isim (false, false, g, g) Q itr_src itr_tgt ths im_src im_tgt st_src st_tgt)
-      (isim (true, true, r, g) Q itr_src itr_tgt ths im_src im_tgt st_src st_tgt)
+      (isim g g Q false false itr_src itr_tgt ths im_src im_tgt st_src st_tgt)
+      (isim r g Q true true itr_src itr_tgt ths im_src im_tgt st_src st_tgt)
   .
   Proof.
     rr. autorewrite with iprop.
@@ -230,7 +252,7 @@ Section SIM.
     :
     bi_entails
       (Q r_src r_tgt ths im_src im_tgt st_src st_tgt)
-      (isim (ps, pt, r, g) Q (Ret r_src) (Ret r_tgt) ths im_src im_tgt st_src st_tgt)
+      (isim r g Q ps pt (Ret r_src) (Ret r_tgt) ths im_src im_tgt st_src st_tgt)
   .
   Proof.
     rr. autorewrite with iprop. i.
@@ -243,8 +265,8 @@ Section SIM.
         itr_src itr_tgt ths im_src im_tgt st_src st_tgt
     :
     bi_entails
-      (isim (true, pt, r, g) Q itr_src itr_tgt ths im_src im_tgt st_src st_tgt)
-      (isim (ps, pt, r, g) Q (Tau itr_src) itr_tgt ths im_src im_tgt st_src st_tgt)
+      (isim r g Q true pt itr_src itr_tgt ths im_src im_tgt st_src st_tgt)
+      (isim r g Q ps pt (Tau itr_src) itr_tgt ths im_src im_tgt st_src st_tgt)
   .
   Proof.
     rr. autorewrite with iprop. i.
@@ -257,8 +279,8 @@ Section SIM.
         itr_src itr_tgt ths im_src im_tgt st_src st_tgt
     :
     bi_entails
-      (isim (ps, true, r, g) Q itr_src itr_tgt ths im_src im_tgt st_src st_tgt)
-      (isim (ps, pt, r, g) Q itr_src (Tau itr_tgt) ths im_src im_tgt st_src st_tgt)
+      (isim r g Q ps true itr_src itr_tgt ths im_src im_tgt st_src st_tgt)
+      (isim r g Q ps pt itr_src (Tau itr_tgt) ths im_src im_tgt st_src st_tgt)
   .
   Proof.
     rr. autorewrite with iprop. i.
@@ -271,8 +293,8 @@ Section SIM.
         ktr_src itr_tgt ths im_src im_tgt st_src st_tgt
     :
     bi_entails
-      (∃ x, isim (true, pt, r, g) Q (ktr_src x) itr_tgt ths im_src im_tgt st_src st_tgt)
-      (isim (ps, pt, r, g) Q (trigger (Choose X) >>= ktr_src) itr_tgt ths im_src im_tgt st_src st_tgt)
+      (∃ x, isim r g Q true pt (ktr_src x) itr_tgt ths im_src im_tgt st_src st_tgt)
+      (isim r g Q ps pt (trigger (Choose X) >>= ktr_src) itr_tgt ths im_src im_tgt st_src st_tgt)
   .
   Proof.
     rr. autorewrite with iprop. i.
@@ -287,8 +309,8 @@ Section SIM.
         itr_src ktr_tgt ths im_src im_tgt st_src st_tgt
     :
     bi_entails
-      (∀ x, isim (ps, true, r, g) Q itr_src (ktr_tgt x) ths im_src im_tgt st_src st_tgt)
-      (isim (ps, pt, r, g) Q itr_src (trigger (Choose X) >>= ktr_tgt) ths im_src im_tgt st_src st_tgt)
+      (∀ x, isim r g Q ps true itr_src (ktr_tgt x) ths im_src im_tgt st_src st_tgt)
+      (isim r g Q ps pt itr_src (trigger (Choose X) >>= ktr_tgt) ths im_src im_tgt st_src st_tgt)
   .
   Proof.
     rr. autorewrite with iprop. i.
@@ -303,8 +325,8 @@ Section SIM.
         ktr_src itr_tgt ths im_src im_tgt st_src st_tgt
     :
     bi_entails
-      (isim (true, pt, r, g) Q (ktr_src tt) itr_tgt ths im_src im_tgt st st_tgt)
-      (isim (ps, pt, r, g) Q (trigger (Put st) >>= ktr_src) itr_tgt ths im_src im_tgt st_src st_tgt)
+      (isim r g Q true pt (ktr_src tt) itr_tgt ths im_src im_tgt st st_tgt)
+      (isim r g Q ps pt (trigger (Put st) >>= ktr_src) itr_tgt ths im_src im_tgt st_src st_tgt)
   .
   Proof.
     rr. autorewrite with iprop. i.
@@ -317,8 +339,8 @@ Section SIM.
         itr_src ktr_tgt ths im_src im_tgt st_src st_tgt
     :
     bi_entails
-      (isim (ps, true, r, g) Q itr_src (ktr_tgt tt) ths im_src im_tgt st_src st)
-      (isim (ps, pt, r, g) Q itr_src (trigger (Put st) >>= ktr_tgt) ths im_src im_tgt st_src st_tgt)
+      (isim r g Q ps true itr_src (ktr_tgt tt) ths im_src im_tgt st_src st)
+      (isim r g Q ps pt itr_src (trigger (Put st) >>= ktr_tgt) ths im_src im_tgt st_src st_tgt)
   .
   Proof.
     rr. autorewrite with iprop. i.
@@ -331,8 +353,8 @@ Section SIM.
         ktr_src itr_tgt ths im_src im_tgt st_src st_tgt
     :
     bi_entails
-      (isim (true, pt, r, g) Q (ktr_src st_src) itr_tgt ths im_src im_tgt st_src st_tgt)
-      (isim (ps, pt, r, g) Q (trigger (@Get _) >>= ktr_src) itr_tgt ths im_src im_tgt st_src st_tgt)
+      (isim r g Q true pt (ktr_src st_src) itr_tgt ths im_src im_tgt st_src st_tgt)
+      (isim r g Q ps pt (trigger (@Get _) >>= ktr_src) itr_tgt ths im_src im_tgt st_src st_tgt)
   .
   Proof.
     rr. autorewrite with iprop. i.
@@ -345,8 +367,8 @@ Section SIM.
         itr_src ktr_tgt ths im_src im_tgt st_src st_tgt
     :
     bi_entails
-      (isim (ps, true, r, g) Q itr_src (ktr_tgt st_tgt) ths im_src im_tgt st_src st_tgt)
-      (isim (ps, pt, r, g) Q itr_src (trigger (@Get _) >>= ktr_tgt) ths im_src im_tgt st_src st_tgt)
+      (isim r g Q ps true itr_src (ktr_tgt st_tgt) ths im_src im_tgt st_src st_tgt)
+      (isim r g Q ps pt itr_src (trigger (@Get _) >>= ktr_tgt) ths im_src im_tgt st_src st_tgt)
   .
   Proof.
     rr. autorewrite with iprop. i.
@@ -359,8 +381,8 @@ Section SIM.
         ktr_src itr_tgt ths im_src im_tgt st_src st_tgt
     :
     bi_entails
-      (isim (true, pt, r, g) Q (ktr_src tid) itr_tgt ths im_src im_tgt st_src st_tgt)
-      (isim (ps, pt, r, g) Q (trigger GetTid >>= ktr_src) itr_tgt ths im_src im_tgt st_src st_tgt)
+      (isim r g Q true pt (ktr_src tid) itr_tgt ths im_src im_tgt st_src st_tgt)
+      (isim r g Q ps pt (trigger GetTid >>= ktr_src) itr_tgt ths im_src im_tgt st_src st_tgt)
   .
   Proof.
     rr. autorewrite with iprop. i.
@@ -373,8 +395,8 @@ Section SIM.
         itr_src ktr_tgt ths im_src im_tgt st_src st_tgt
     :
     bi_entails
-      (isim (ps, true, r, g) Q itr_src (ktr_tgt tid) ths im_src im_tgt st_src st_tgt)
-      (isim (ps, pt, r, g) Q itr_src (trigger GetTid >>= ktr_tgt) ths im_src im_tgt st_src st_tgt)
+      (isim r g Q ps true itr_src (ktr_tgt tid) ths im_src im_tgt st_src st_tgt)
+      (isim r g Q ps pt itr_src (trigger GetTid >>= ktr_tgt) ths im_src im_tgt st_src st_tgt)
   .
   Proof.
     rr. autorewrite with iprop. i.
@@ -387,8 +409,8 @@ Section SIM.
         ktr_src itr_tgt ths im_src0 im_tgt st_src st_tgt
     :
     bi_entails
-      (∃ im_src1, ⌜fair_update im_src0 im_src1 f⌝ ∧ isim (true, pt, r, g) Q (ktr_src tt) itr_tgt ths im_src1 im_tgt st_src st_tgt)
-      (isim (ps, pt, r, g) Q (trigger (Fair f) >>= ktr_src) itr_tgt ths im_src0 im_tgt st_src st_tgt)
+      (∃ im_src1, ⌜fair_update im_src0 im_src1 f⌝ ∧ isim r g Q true pt (ktr_src tt) itr_tgt ths im_src1 im_tgt st_src st_tgt)
+      (isim r g Q ps pt (trigger (Fair f) >>= ktr_src) itr_tgt ths im_src0 im_tgt st_src st_tgt)
   .
   Proof.
     rr. autorewrite with iprop. i.
@@ -405,8 +427,8 @@ Section SIM.
         itr_src ktr_tgt ths im_src im_tgt0 st_src st_tgt
     :
     bi_entails
-      (∀ im_tgt1, ⌜fair_update im_tgt0 im_tgt1 (sum_fmap_r f)⌝ -* isim (ps, true, r, g) Q itr_src (ktr_tgt tt) ths im_src im_tgt1 st_src st_tgt)
-      (isim (ps, pt, r, g) Q itr_src (trigger (Fair f) >>= ktr_tgt) ths im_src im_tgt0 st_src st_tgt)
+      (∀ im_tgt1, ⌜fair_update im_tgt0 im_tgt1 (sum_fmap_r f)⌝ -* isim r g Q ps true itr_src (ktr_tgt tt) ths im_src im_tgt1 st_src st_tgt)
+      (isim r g Q ps pt itr_src (trigger (Fair f) >>= ktr_tgt) ths im_src im_tgt0 st_src st_tgt)
   .
   Proof.
     rr. autorewrite with iprop. i.
@@ -427,7 +449,7 @@ Section SIM.
     :
     bi_entails
       (True)
-      (isim (ps, pt, r, g) Q (trigger Undefined >>= ktr_src) itr_tgt ths im_src im_tgt st_src st_tgt)
+      (isim r g Q ps pt (trigger Undefined >>= ktr_src) itr_tgt ths im_src im_tgt st_src st_tgt)
   .
   Proof.
     rr. autorewrite with iprop. i.
@@ -440,8 +462,8 @@ Section SIM.
         ktr_src ktr_tgt ths im_src im_tgt st_src st_tgt
     :
     bi_entails
-      (∀ ret, isim (true, true, g, g) Q (ktr_src ret) (ktr_tgt ret) ths im_src im_tgt st_src st_tgt)
-      (isim (ps, pt, r, g) Q (trigger (Observe fn args) >>= ktr_src) (trigger (Observe fn args) >>= ktr_tgt) ths im_src im_tgt st_src st_tgt)
+      (∀ ret, isim g g Q true true (ktr_src ret) (ktr_tgt ret) ths im_src im_tgt st_src st_tgt)
+      (isim r g Q ps pt (trigger (Observe fn args) >>= ktr_src) (trigger (Observe fn args) >>= ktr_tgt) ths im_src im_tgt st_src st_tgt)
   .
   Proof.
     rr. autorewrite with iprop. i.
@@ -456,8 +478,8 @@ Section SIM.
         ktr_src ktr_tgt ths im_src im_tgt st_src st_tgt
     :
     bi_entails
-      (isim (true, pt, r, g) Q (ktr_src tt) (trigger (Yield) >>= ktr_tgt) ths im_src im_tgt st_src st_tgt)
-      (isim (ps, pt, r, g) Q (trigger (Yield) >>= ktr_src) (trigger (Yield) >>= ktr_tgt) ths im_src im_tgt st_src st_tgt)
+      (isim r g Q true pt (ktr_src tt) (trigger (Yield) >>= ktr_tgt) ths im_src im_tgt st_src st_tgt)
+      (isim r g Q ps pt (trigger (Yield) >>= ktr_src) (trigger (Yield) >>= ktr_tgt) ths im_src im_tgt st_src st_tgt)
   .
   Proof.
     rr. autorewrite with iprop. i.
@@ -470,8 +492,8 @@ Section SIM.
         ktr_src ktr_tgt ths0 im_src0 im_tgt0 st_src0 st_tgt0
     :
     bi_entails
-      (I ths0 im_src0 im_tgt0 st_src0 st_tgt0 ** (∀ ths1 im_src1 im_tgt1 st_src1 st_tgt1 im_tgt2, I ths1 im_src1 im_tgt1 st_src1 st_tgt1 -* ⌜fair_update im_tgt1 im_tgt2 (sum_fmap_l (tids_fmap tid ths1))⌝ -* isim (ps, true, r, g) Q (trigger (Yield) >>= ktr_src) (ktr_tgt tt) ths1 im_src1 im_tgt2 st_src1 st_tgt1))
-      (isim (ps, pt, r, g) Q (trigger (Yield) >>= ktr_src) (trigger (Yield) >>= ktr_tgt) ths0 im_src0 im_tgt0 st_src0 st_tgt0)
+      (I ths0 im_src0 im_tgt0 st_src0 st_tgt0 ** (∀ ths1 im_src1 im_tgt1 st_src1 st_tgt1 im_tgt2, I ths1 im_src1 im_tgt1 st_src1 st_tgt1 -* ⌜fair_update im_tgt1 im_tgt2 (sum_fmap_l (tids_fmap tid ths1))⌝ -* isim r g Q ps true (trigger (Yield) >>= ktr_src) (ktr_tgt tt) ths1 im_src1 im_tgt2 st_src1 st_tgt1))
+      (isim r g Q ps pt (trigger (Yield) >>= ktr_src) (trigger (Yield) >>= ktr_tgt) ths0 im_src0 im_tgt0 st_src0 st_tgt0)
   .
   Proof.
     rr. autorewrite with iprop. i.
@@ -498,8 +520,8 @@ Section SIM.
         ktr_src ktr_tgt ths0 im_src0 im_tgt0 st_src0 st_tgt0
     :
     bi_entails
-      (I ths0 im_src0 im_tgt0 st_src0 st_tgt0 ** (∀ ths1 im_src1 im_tgt1 st_src1 st_tgt1 im_tgt2, I ths1 im_src1 im_tgt1 st_src1 st_tgt1 -* ⌜fair_update im_tgt1 im_tgt2 (sum_fmap_l (tids_fmap tid ths1))⌝ -* isim (true, true, g, g) Q (ktr_src tt) (ktr_tgt tt) ths1 im_src1 im_tgt2 st_src1 st_tgt1))
-      (isim (ps, pt, r, g) Q (trigger (Yield) >>= ktr_src) (trigger (Yield) >>= ktr_tgt) ths0 im_src0 im_tgt0 st_src0 st_tgt0)
+      (I ths0 im_src0 im_tgt0 st_src0 st_tgt0 ** (∀ ths1 im_src1 im_tgt1 st_src1 st_tgt1 im_tgt2, I ths1 im_src1 im_tgt1 st_src1 st_tgt1 -* ⌜fair_update im_tgt1 im_tgt2 (sum_fmap_l (tids_fmap tid ths1))⌝ -* isim g g Q true true (ktr_src tt) (ktr_tgt tt) ths1 im_src1 im_tgt2 st_src1 st_tgt1))
+      (isim r g Q ps pt (trigger (Yield) >>= ktr_src) (trigger (Yield) >>= ktr_tgt) ths0 im_src0 im_tgt0 st_src0 st_tgt0)
   .
   Proof.
     rr. autorewrite with iprop. i.
@@ -520,71 +542,62 @@ Section SIM.
     i. eapply H2. r_wf VALID.
   Qed.
 
-  Variant unlift2 (r: rel):
-    forall R_src R_tgt (RR: R_src -> R_tgt -> Σ ->
-                            (TIdSet.t *
-                               (@imap ident_src wf_src) *
-                               (@imap (sum_tid ident_tgt) nat_wf) *
-                               state_src *
-                               state_tgt) -> Prop),
-      bool -> bool -> Σ -> itree srcE R_src -> itree tgtE R_tgt ->
-      (TIdSet.t *
-         (@imap ident_src wf_src) *
-         (@imap (sum_tid ident_tgt) nat_wf) *
-         state_src *
-         state_tgt) -> Prop :=
-    | unlift2_intro
-        ps pt
-        R_src R_tgt Q itr_src itr_tgt ths im_src im_tgt st_src st_tgt r_ctx r_own
-        (REL: r R_src R_tgt Q itr_src itr_tgt ths im_src im_tgt st_src st_tgt r_own)
-        (WF: URA.wf (r_own ⋅ r_ctx))
-      :
-      unlift2 r (liftRR Q) ps pt r_ctx itr_src itr_tgt (ths, im_src, im_tgt, st_src, st_tgt)
-  .
-
   Lemma isim_base ps pt r g R_src R_tgt
         (Q: R_src -> R_tgt -> shared_rel)
         itr_src itr_tgt ths im_src im_tgt st_src st_tgt
     :
     bi_entails
-      (@r _ _ Q itr_src itr_tgt ths im_src im_tgt st_src st_tgt)
-      (isim (ps, pt, r, g) Q itr_src itr_tgt ths im_src im_tgt st_src st_tgt)
+      (@r _ _ Q ps pt itr_src itr_tgt ths im_src im_tgt st_src st_tgt)
+      (isim r g Q ps pt itr_src itr_tgt ths im_src im_tgt st_src st_tgt)
   .
   Proof.
     rr. autorewrite with iprop.
-    ii. gbase.
+    ii. gbase. econs; eauto.
+  Qed.
 
-    unfold liftRR. rr. esplits. eauto.
-
-  (* H : r R_src R_tgt Q itr_src itr_tgt ths im_src im_tgt st_src st_tgt r0 *)
-  (* r_ctx : Σ *)
-  (* WF0 : URA.wf (r0 ⋅ r_ctx) *)
-  (* ============================ *)
-  (* unlift r (liftRR Q) ps pt r_ctx itr_src itr_tgt *)
-  (*   (ths, im_src, im_tgt, st_src, st_tgt) *)
-
-  Admitted.
+  Lemma unlift_mon (r0 r1: rel)
+        (MON: forall R_src R_tgt (Q: R_src -> R_tgt -> shared_rel)
+                     ps pt itr_src itr_tgt ths im_src im_tgt st_src st_tgt,
+            bi_entails
+              (@r0 _ _ Q ps pt itr_src itr_tgt ths im_src im_tgt st_src st_tgt)
+              (#=> (@r1 _ _ Q ps pt itr_src itr_tgt ths im_src im_tgt st_src st_tgt)))
+    :
+    unlift2 r0 <9= unlift2 r1.
+  Proof.
+    i. dependent destruction PR.
+    hexploit MON; eauto. i.
+    rr in H. autorewrite with iprop in H.
+    hexploit H; [|eauto|..].
+    { eapply URA.wf_mon. eauto. }
+    i. rr in H0. autorewrite with iprop in H0.
+    hexploit H0; eauto. i. des. econs; eauto.
+  Qed.
 
   Lemma isim_mono_knowledge (r0 g0 r1 g1: rel) ps pt R_src R_tgt
         (Q: R_src -> R_tgt -> shared_rel)
         itr_src itr_tgt ths im_src im_tgt st_src st_tgt
         (MON0: forall R_src R_tgt (Q: R_src -> R_tgt -> shared_rel)
-                      itr_src itr_tgt ths im_src im_tgt st_src st_tgt,
+                      ps pt itr_src itr_tgt ths im_src im_tgt st_src st_tgt,
             bi_entails
-              (@r0 _ _ Q itr_src itr_tgt ths im_src im_tgt st_src st_tgt)
-              (#=> (@r1 _ _ Q itr_src itr_tgt ths im_src im_tgt st_src st_tgt)))
+              (@r0 _ _ Q ps pt itr_src itr_tgt ths im_src im_tgt st_src st_tgt)
+              (#=> (@r1 _ _ Q ps pt itr_src itr_tgt ths im_src im_tgt st_src st_tgt)))
         (MON1: forall R_src R_tgt (Q: R_src -> R_tgt -> shared_rel)
-                      itr_src itr_tgt ths im_src im_tgt st_src st_tgt,
+                      ps pt itr_src itr_tgt ths im_src im_tgt st_src st_tgt,
             bi_entails
-              (@g0 _ _ Q itr_src itr_tgt ths im_src im_tgt st_src st_tgt)
-              (#=> (@g1 _ _ Q itr_src itr_tgt ths im_src im_tgt st_src st_tgt)))
+              (@g0 _ _ Q ps pt itr_src itr_tgt ths im_src im_tgt st_src st_tgt)
+              (#=> (@g1 _ _ Q ps pt itr_src itr_tgt ths im_src im_tgt st_src st_tgt)))
     :
     bi_entails
-      (isim (ps, pt, r0, g0) Q itr_src itr_tgt ths im_src im_tgt st_src st_tgt)
-      (isim (ps, pt, r1, g1) Q itr_src itr_tgt ths im_src im_tgt st_src st_tgt)
+      (isim r0 g0 Q ps pt itr_src itr_tgt ths im_src im_tgt st_src st_tgt)
+      (isim r1 g1 Q ps pt itr_src itr_tgt ths im_src im_tgt st_src st_tgt)
   .
   Proof.
-  Admitted.
+    rr. autorewrite with iprop. i.
+    ii. rr in H. hexploit H; eauto. i.
+    eapply gpaco9_mon; eauto.
+    { eapply unlift_mon; eauto. }
+    { eapply unlift_mon; eauto. }
+  Qed.
 
   Ltac espc H :=
     let T := fresh "T" in
@@ -596,112 +609,34 @@ Section SIM.
   Tactic Notation "rspc" constr(H) := rr in H; autorewrite with iprop in H; espc H.
   Ltac rspc := rr; autorewrite with iprop.
 
-  Lemma unlift_mon (r0 r1: rel)
-        (MON: forall R_src R_tgt (Q: R_src -> R_tgt -> shared_rel)
-                     itr_src itr_tgt ths im_src im_tgt st_src st_tgt,
-            bi_entails
-              (@r0 _ _ Q itr_src itr_tgt ths im_src im_tgt st_src st_tgt)
-              (#=> (@r1 _ _ Q itr_src itr_tgt ths im_src im_tgt st_src st_tgt)))
-    :
-    unlift r0 <9= unlift r1.
-  Admitted.
-
-  Lemma isim_coind' A
-        (ps: forall (a: A), bool)
-        (pt: forall (a: A), bool)
-        (R_src: forall (a: A), Prop)
-        (R_tgt: forall (a: A), Prop)
-        (Q: forall (a: A), R_src a -> R_tgt a -> shared_rel)
-        (itr_src : forall (a: A), itree srcE (R_src a))
-        (itr_tgt : forall (a: A), itree tgtE (R_tgt a))
-        (ths: forall (a: A), TIdSet.t)
-        (im_src: forall (a: A), imap ident_src wf_src)
-        (im_tgt: forall (a: A), imap (sum_tid ident_tgt) nat_wf)
-        (st_src: forall (a: A), state_src)
-        (st_tgt: forall (a: A), state_tgt)
-        (P: forall (a: A), iProp)
-        (r g0: rel)
-    :
-    bi_entails
-      (∀ (g1: rel) a,
-          P a -*
-            (□(∀ R_src R_tgt (Q: R_src -> R_tgt -> shared_rel)
-                itr_src itr_tgt ths im_src im_tgt st_src st_tgt,
-                 @g0 R_src R_tgt Q itr_src itr_tgt ths im_src im_tgt st_src st_tgt -* @g1 R_src R_tgt Q itr_src itr_tgt ths im_src im_tgt st_src st_tgt)) -*
-            (□(∀ a,
-                 P a -* @g1 (R_src a) (R_tgt a) (Q a) (itr_src a) (itr_tgt a) (ths a) (im_src a) (im_tgt a) (st_src a) (st_tgt a))) -*
-            isim (ps a, pt a, r, g1) (Q a) (itr_src a) (itr_tgt a) (ths a) (im_src a) (im_tgt a) (st_src a) (st_tgt a))
-      (∀ a, P a -* isim (ps a, pt a, r, g0) (Q a) (itr_src a) (itr_tgt a) (ths a) (im_src a) (im_tgt a) (st_src a) (st_tgt a))
-  .
+  Goal forall (A B C: iProp),
+      bi_entails
+        (□ A)
+        A.
   Proof.
-    rr. autorewrite with iprop. i.
-    rr. autorewrite with iprop. i.
-    rr. autorewrite with iprop.
-    revert x. gcofix CIH. i. eapply gpaco9_gpaco.
-    { auto with paco. }
-    epose (fun R_src R_tgt (Q: R_src -> R_tgt -> shared_rel)
-               itr_src itr_tgt ths im_src im_tgt st_src st_tgt =>
-             @iProp_intro _ (fun r_own => forall r_ctx (WF: URA.wf (r_own ⋅ r_ctx)),
-                                 gpaco9 gf (cpn9 gf) r1 r1 R_src R_tgt (liftRR Q) false false r_ctx itr_src itr_tgt (ths, im_src, im_tgt, st_src, st_tgt)) _).
-    rr in H. autorewrite with iprop in H. specialize (H i). subst i.
-    rspc H.
-    rr in H. autorewrite with iprop in H.
-    hexploit H; eauto. clear H. i.
-    rr in H. autorewrite with iprop in H.
-    hexploit (H URA.unit); eauto.
-    { r_wf H1. }
-    { rr. autorewrite with iprop. split.
-      { rr. autorewrite with iprop. auto. }
-      rr. autorewrite with iprop.
-      do 11 (rr; autorewrite with iprop; i).
-      rewrite URA.unit_core. rewrite URA.unit_idl.
-      ss. i. gbase. eapply CIH0.
-      (* rr. esplits. eauto. eauto. *)
-
-      (* rr in H3. autorewrite with iprop in H3. *)
-      (* hexploit H3; eauto. i. des. *)
-
-
-      (* muclo lsim_monoC_spec. econs. *)
-      (* 2:{ gbase. eapply CIH0. *)
-      (*     rr. esplits. eauto. eauto. *)
-
-      (* g0 x0 x1 x2 x3 x4 x5 x6 x7 x8 x9 rp0 -> forall r_ctx (WF: URA.wf (rp0 ⋅ r_ctx0)), unlift g0 (liftRR x2) false false r_ctx0 x3 x4 (x5, x6, x7, x8, x9) *)
-      admit.
-    } clear H.
-    i. rr in H. autorewrite with iprop in H.
-    hexploit (H URA.unit); eauto.
-    { r_wf H1. }
-    { rr. autorewrite with iprop. split.
-      { rr. autorewrite with iprop. auto. }
-      rr. autorewrite with iprop.
-      do 2 (rr; autorewrite with iprop; i).
-      rewrite URA.unit_core. rewrite URA.unit_idl.
-      ss. i.
-      hexploit CIH.
-      2:{ eauto. }
-      { admit. }
-      { admit. }
-      i. muclo lsim_resetC_spec. econs.
-      { gbase. eauto. }
-      { admit. }
-      { admit. }
-    }
-    i. eapply gpaco9_mon.
-    { eapply H0. r_wf WF0. }
-    { i. gbase. eauto. }
-    { i. gbase. left. eapply CIH0.
-      eapply unlift_mon; [|eauto].
-      i. ss. rr. autorewrite with iprop. i.
-      ss. rr. autorewrite with iprop. i.
-      esplits. eauto.
-
-
-
-      rr. eapply
-      admit. }
+    i. iIntros "#H". iApply "H".
   Qed.
 
+  Goal forall (A B C: iProp),
+      bi_entails
+        (□ (A -* B))
+        (□ (A → B))
+  .
+  Proof.
+    i. iIntros "#H". iModIntro.
+    iIntros "X". iApply "H". iApply "X".
+  Qed.
+
+  Goal forall (A B C: iProp),
+      bi_entails
+        (A → B)
+        (A -* B).
+  Proof.
+    i. iIntros "X Y".
+    iAssert (A ∧ (A → B))%I with "[X Y]" as "XX".
+    { iSplit; auto. }
+    iApply bi.impl_elim_r. eauto.
+  Qed.
 
   Lemma isim_coind A
         (ps: forall (a: A), bool)
@@ -718,120 +653,46 @@ Section SIM.
         (st_tgt: forall (a: A), state_tgt)
         (P: forall (a: A), iProp)
         (r g0: rel)
+        (COIND: forall (g1: rel) a, bi_entails (□((∀ R_src R_tgt (Q: R_src -> R_tgt -> shared_rel)
+                                                     ps pt itr_src itr_tgt ths im_src im_tgt st_src st_tgt,
+                                                      @g0 R_src R_tgt Q ps pt itr_src itr_tgt ths im_src im_tgt st_src st_tgt -* @g1 R_src R_tgt Q ps pt itr_src itr_tgt ths im_src im_tgt st_src st_tgt)
+                                                    **
+                                                    (∀ a, P a -* @g1 (R_src a) (R_tgt a) (Q a) (ps a) (pt a) (itr_src a) (itr_tgt a) (ths a) (im_src a) (im_tgt a) (st_src a) (st_tgt a))) ** P a) (isim r g0 (Q a) (ps a) (pt a) (itr_src a) (itr_tgt a) (ths a) (im_src a) (im_tgt a) (st_src a) (st_tgt a)))
     :
-    bi_entails
-      (∀ (g1: rel) a,
-          P a -*
-            (□(∀ R_src R_tgt (Q: R_src -> R_tgt -> shared_rel)
-                itr_src itr_tgt ths im_src im_tgt st_src st_tgt,
-                 @g0 R_src R_tgt Q itr_src itr_tgt ths im_src im_tgt st_src st_tgt -* @g1 R_src R_tgt Q itr_src itr_tgt ths im_src im_tgt st_src st_tgt)) -*
-            (□(∀ a,
-                 P a -* @g1 (R_src a) (R_tgt a) (Q a) (itr_src a) (itr_tgt a) (ths a) (im_src a) (im_tgt a) (st_src a) (st_tgt a))) -*
-            isim (ps a, pt a, r, g1) (Q a) (itr_src a) (itr_tgt a) (ths a) (im_src a) (im_tgt a) (st_src a) (st_tgt a))
-      (∀ a, P a -* isim (ps a, pt a, r, g0) (Q a) (itr_src a) (itr_tgt a) (ths a) (im_src a) (im_tgt a) (st_src a) (st_tgt a))
-  .
+    (forall a, bi_entails (P a) (isim r g0 (Q a) (ps a) (pt a) (itr_src a) (itr_tgt a) (ths a) (im_src a) (im_tgt a) (st_src a) (st_tgt a))).
   Proof.
-    rr. autorewrite with iprop. i.
-    rr. autorewrite with iprop. i.
-    rr. autorewrite with iprop.
-    revert x. gcofix CIH. i.
-    rspc H. rspc H.
-    rr in H. autorewrite with iprop in H.
-    hexploit H; eauto. clear H. i.
-    rr in H. autorewrite with iprop in H.
-    hexploit (H URA.unit); eauto.
-    { r_wf H1. }
-    { rr. autorewrite with iprop. split.
-      { rr. autorewrite with iprop. auto. }
+    i. rr. autorewrite with iprop. ii. clear WF.
+    revert a r0 H r_ctx WF0. gcofix CIH. i.
+    epose (fun R_src R_tgt (Q: R_src -> R_tgt -> shared_rel)
+               ps pt itr_src itr_tgt ths im_src im_tgt st_src st_tgt =>
+             @iProp_intro _ (fun r_own => forall r_ctx (WF: URA.wf (r_own ⋅ r_ctx)),
+                                 gpaco9 gf (cpn9 gf) r0 r0 R_src R_tgt (liftRR Q) ps pt r_ctx itr_src itr_tgt (ths, im_src, im_tgt, st_src, st_tgt)) _).
+    hexploit (COIND i a). subst i. clear COIND. i.
+    rr in H. autorewrite with iprop in H. hexploit H.
+    { instantiate (1:=r1). eapply URA.wf_mon; eauto. }
+    { rr. autorewrite with iprop.
+      exists URA.unit, r1. splits; auto.
+      { r_solve. }
+      rr. autorewrite with iprop. esplits.
+      { rr. autorewrite with iprop. ss. }
       rr. autorewrite with iprop.
-      do 11 (rr; autorewrite with iprop; i).
-      rewrite URA.unit_core. rewrite URA.unit_idl.
-      instantiate (1:=fun R_src R_tgt (Q: R_src -> R_tgt -> shared_rel)
-                          itr_src itr_tgt ths im_src im_tgt st_src st_tgt =>
-                        r1 ? false false
-                  ).
-
-      instantiate (1:=lift r1).
-      eapply H3.
-
-    } clear H.
-    i. rr in H. autorewrite with iprop in H.
-    hexploit (H URA.unit); eauto.
-    { r_wf H1. }
-    { rr. autorewrite with iprop. split.
-      { rr. autorewrite with iprop. auto. }
       rr. autorewrite with iprop.
-      do 2 (rr; autorewrite with iprop; i).
-      rewrite URA.unit_core. rewrite URA.unit_idl.
-      admit.
+      exists URA.unit, URA.unit. splits.
+      { rewrite URA.unit_core. r_solve. }
+      { do 13 (rr; autorewrite with iprop; i).
+        ss. i. gbase. eapply CIH0. econs; eauto. r_wf WF.
+      }
+      { do 2 (rr; autorewrite with iprop; i).
+        ss. i. gbase. eapply CIH; eauto. r_wf WF.
+      }
     }
-    i. eapply gpaco9_mon.
-    { eapply H0. r_wf WF0. }
-    { i. eauto. }
-    { eapply CIH0. }
-  Qed.
-
-    rr in H0. eapply gpaco9_mon.
-    { eapply H0.
-
-
-    eapply H0.
-
-    i.
-
-    {
-
-
-
-
-ss.      rewrite URA.unit_id.
-
-      rr. autorewrite with iprop. i.
-      rr. autorewrite with iprop. i.
-      rr. autorewrite with iprop. i.
-      rr. autorewrite with iprop. i.
-      rr. autorewrite with iprop. i.
-      rr. autorewrite with iprop. i.
-      rr. autorewrite with iprop. i.
-      rr. autorewrite with iprop. i.
-      rr. autorewrite with iprop. i.
-      r
-
-      split.
-      {
-
-
-      instantiate (1:=r1).
-
-      instantiate (1:=r1).
-
-    2:{
-      i. rr in H0. autorewrite with iprop in H0.
-      hexploit H0.
-
-    clear H. i.
-
-    ; [|eauto|..]; eauto. clear H. i.
-
-
-
-    { admit. }
+    clear H. i. eapply gpaco9_mon.
+    { eapply H. eauto. }
     { eauto. }
-
-
-    espc H.
-    rr in H. autorewrite with iprop in H. espc H.
-    rr in H.
-
-    ;
-
-
-      evar (T: Type).
-    specialize (H
-    s
-
-    i.
-
-
-  Admitted.
+    { i. eauto. }
+    Unshelve.
+    { i. ss. i. eapply H; eauto.
+      eapply URA.wf_extends; eauto. eapply URA.extends_add; eauto.
+    }
+  Qed.
 End SIM.
